stronger version of the square diagram

src/PL.v
@@ -453,24 +453,52 @@ Section Concretization.
       assumption.
   Qed.
 
+  (* This hypothesis is necessary to prove that the diagram commutes with dereference, it should be a consequence that the PL_state Spl is the concretization of the HLPL state S *)
   Definition addresses_are_compatible (S : HLPL_state) (Spl : PL_state) :=
-    forall bi off t p l,
-      addr_spath_equiv S ((bi, off), t) p ->
-      get_node (S.[p]) = locC(l) ->
-      addrof l = Some (bi, off).
+    forall S addr addr' t sp l,
+      addr_spath_equiv S (addr, (TRef t)) sp ->
+      get_node (S.[ sp ]) = ptrC(l) ->
+      lookup_heap_at_addr addr (TRef t) Spl = [PL_address addr'] ->
+      addrof l = Some addr'.
 
   Lemma addr_spath_deref_proj (S : HLPL_state) (Spl : PL_state) :
-    forall bi off bi' off' x pi y pi' t perm,
+    forall bi bi' off off' x y pi pi' t perm,
       addresses_are_compatible S Spl ->
       addr_spath_equiv S ((bi, off), TRef t) (x, pi) ->
       eval_proj S perm Deref (x, pi) (y, pi') ->
       eval_proj_addr Spl Deref ((bi, off), TRef t) ((bi', off'), t) ->
       addr_spath_equiv S ((bi', off'), t) (y, pi').
   Proof.
-    intros bi off bi' off' x pi y pi' t perm Haddrcomp Hequiv Hproj Hprojaddr.
+    intros bi bi' off off' x y pi pi' t perm Haddrcomp Hequiv Hproj Hprojaddr.
     inversion Hproj ; subst ; inversion Hprojaddr ; subst.
     eapply Addr_spath_pointer ; try eassumption.
+    unfold addresses_are_compatible in Haddrcomp.
+    apply Haddrcomp with (S := S) (addr := (bi, off)) (t := t) (sp := (x, pi)) ;
+      try assumption.
+    simpl. rewrite Haddr. rewrite <- hd_error_skipn in Hoff.
+    destruct (drop off pl) eqn:E.
+    * discriminate.
+    * simpl in Hoff. injection Hoff ; intros ; subst.
+      auto.
+  Qed.
 
+
+  (* The commuting diagram to relate addresses and spath *)
+  Lemma addr_spath_proj (S : HLPL_state) (Spl : PL_state) :
+    forall proj bi bi' off off' x y pi pi' t t' perm,
+      addresses_are_compatible S Spl ->
+      addr_spath_equiv S ((bi, off), t) (x, pi) ->
+      eval_proj S perm proj (x, pi) (y, pi') ->
+      eval_proj_addr Spl proj ((bi, off), t) ((bi', off'), t') ->
+      addr_spath_equiv S ((bi', off'), t') (y, pi').
+  Proof.
+    intros [ | ]
+      bi bi' off off' x y pi pi' t t' perm Haddrcomp Hequiv Hproj Hprojaddr.
+    * inversion Hproj ; subst ; inversion Hprojaddr ; subst.
+      eapply addr_spath_deref_proj ; eassumption.
+    * inversion Hproj ; subst ; inversion Hprojaddr ; subst ; inversion H3 ; subst ;
+        eapply addr_spath_pair_proj ; eauto.
+  Qed.
 
 Lemma concr_val_TInt_implies_PL_int :
     forall v vl, concr_hlpl_val v TInt vl -> (exists n, vl = [PL_int n]) \/ vl = [PL_poison].
@@ -509,24 +537,6 @@ Lemma concr_val_TInt_implies_PL_int :
       + admit.
     - admit.
     - 
-  Abort.
-
-  Lemma addr_spath_deref_proj (S : HLPL_state) (Spl : PL_state) :
-    forall bi bi' off off' x y pi pi' t perm,
-      le_pl_hlpl Spl S ->
-      addr_spath_equiv S ((bi, off), TRef t) (x, pi) ->
-      eval_proj S perm Deref (x, pi) (y, pi') ->
-      eval_proj_addr Spl Deref ((bi, off), TRef t) ((bi', off'), t) ->
-      addr_spath_equiv S ((bi', off'), t) (y, pi').
-  Proof.
-    intros ? ? ? ? ? ? ? ? ? ?
-      [ Spl' [ [Hdom Haddr Hreach ] [[ Hconcr_heap Hconcr_env] Hle] ] ]
-      Hequi Hproj Hprojaddr.
-    inversion Hproj ; subst. eapply Addr_spath_pointer.
-    - apply get_q'.
-    - apply get_q.
-    - apply Hequi. 
-    - inversion Hprojaddr ; subst.
   Abort.
       
 End Concretization.
